Added XOR instruction and proofs.

src/coq/App/Instruction.v
@@ -14,7 +14,8 @@ Inductive Instruction : Type :=
     | SHL : nat -> Instruction
     | SHR : nat -> Instruction
     | AND : Instruction
-    | OR : Instruction.
+    | OR : Instruction
+    | XOR : Instruction.
 
 (* The time to execute a NOP instruction. *)
 Definition NOP_DELAY : nat := 1.
@@ -42,5 +43,8 @@ Definition AND_DELAY : nat := 2.
 
 (* The time to execute an OR instruction. *)
 Definition OR_DELAY : nat := 2.
+
+(* The time to execute an XOR instruction. *)
+Definition XOR_DELAY : nat := 2.
 
 End Instruction.
