src/coq/Data/Bits.v
@@ -28,8 +28,11 @@ Definition Z_to_B64 (z : Z) : B64 := Z_to_binary 64 z.
 (* Perform an AND operation on two BV64 values. *)
 Definition B64_and (x y : B64) : B64 := BVand 64 x y.
 
-(* Perform an AND operation on two BV64 values. *)
+(* Perform an OR operation on two BV64 values. *)
 Definition B64_or (x y : B64) : B64 := BVor 64 x y.
+
+(* Perform an XOR operation on two BV64 values. *)
+Definition B64_xor (x y : B64) : B64 := BVxor 64 x y.
 
 Module ZStuff.
 
